restored ported version of shrink_cps

certicoq/theories/L6_PCPS/shrink_cps.v
@@ -11,9 +11,11 @@ Import Nnat.
 Require Import Coq.Arith.Arith Coq.NArith.BinNat ExtLib.Data.String ExtLib.Data.List Coq.omega.Omega Coq.Program.Program Coq.micromega.Psatz.
 Require Import CpdtTactics Coq.Sorting.Permutation.
 Require Import HashMap.
-Require Import cps.
-Require Import cps_util.
 Require Import maps_util.
+Require Import cps.
+Require Import ctx.
+Require Import cps_util.
+
 
 Definition var_dec := M.elt_eq.
 
@@ -29,8 +31,6 @@ Definition ctx_map := M.t value.
 (* renamer maps x |-> a *)
 Definition r_map := M.t var.
 
-(* census2 maps x |-> # applied occurrences, # escaping occurrences *)
-Definition c2_map := M.t (nat * nat).
 
 (* census maps x |-> total # of occurences *)
 Definition c_map :=  M.t nat.
@@ -42,15 +42,15 @@ Definition getd {A:Type} (d:A) :=
                | None => d
                | Some e => e
                end.
+
 Definition seto {A:Type} (x:var)(oa:option A) (map:M.t A):=
   match oa with
   | Some a => M.set x a map
   | None => map
   end.
 
-Definition get_c2 := getd (0,0).
-Definition get_c := getd 0.
-Definition get_b := getd false.
+Notation get_c := (getd 0%nat).
+Notation get_b := (getd false).
 
 
   Fixpoint get_fun (f:var) (fds:fundefs): option (type * list var * exp) :=
@@ -66,11 +66,12 @@ Section MEASURECONTRACT.
 
   Create HintDb mtss.
   
-  (* compute the tree height of an expression *)
+  (* compute the number of constructors of an expression *)
   Fixpoint term_size (e: exp) : nat :=
     match e with
       | Econstr _ _ _ _ e => 1 + term_size e
-      | Ecase _ cl => 1 + length cl
+      | Ecase _ cl => 1 + (List.fold_right (fun (p:(var * exp)) => fun  (n:nat)  => let (k, e) := p in
+                                                                               (n + (term_size e))%nat) 0%nat cl)
       | Eproj _ _ _ _ e => 1 + term_size e
       | Eapp _ _ => 1
       | Eprim _ _ _ _ e => 1 + term_size e
@@ -89,29 +90,22 @@ Section MEASURECONTRACT.
     | Vfun t lv e =>  1 + term_size e 
     end.
   
+  
   Theorem subterm_size : forall e e',
-                           subterm_e e' e -> term_size e' < term_size e
+                           subterm_e e' e -> (term_size e' < term_size e)%nat
                            with subterm_fds_size: forall e fds,
-                           subterm_fds_e e fds -> term_size e < funs_size fds                         
+                           subterm_fds_e e fds -> (term_size e < funs_size fds)%nat
   .
   Proof.
-    - induction e; intros. 
-     + inversion H; subst; [simpl; omega | simpl; apply subterm_size in H2;  omega].  
-     + inversion H.
-     + inversion H; subst; [simpl; omega | simpl; apply subterm_size in H2;  omega]. 
-     + inversion H; subst. simpl. rewrite plus_n_Sm. apply subterm_fds_size in H2. omega.
-     + inversion H; subst. 
-     + inversion H; subst; [simpl; omega | simpl; apply subterm_size in H2;  omega]. 
-    - intros. inversion H; subst. simpl. omega. simpl. apply subterm_size in H0. omega.  apply subterm_fds_size in H. assumption.
- Admitted. 
+  Admitted.
 
 
   Definition fold1r (A B : Type) (f: A -> B -> B) (sub:M.t A) (b:B): B  :=
     List.fold_right (fun p a => f (snd p) a) b (M.elements sub).
 
-  
+
   Definition sub_size (sub: ctx_map) : nat :=
-   fold1r _ _ (fun v => fun n => (value_size v) + n) sub 0.
+   (fold1r _ _ (fun v => fun n => (value_size v) + n) sub 0)%nat.
 
 
 
@@ -149,7 +143,7 @@ Admitted.
     
     
     Theorem sub_remove_size: forall x v sub, M.get x sub = Some v ->
-                                             sub_size (M.remove x sub) + value_size v = sub_size sub.
+                                             (sub_size (M.remove x sub) + value_size v = sub_size sub)%nat.
   Proof. 
     intros. unfold sub_size. unfold fold1r.  apply elements_remove in H. do 3 destruct H.  rewrite H0. rewrite H.   rewrite SetoidList.fold_right_commutes. apply plus_comm. apply equiv_size_eq. crush. intro. intros. intro. intros. unfold equiv_size in H1. subst. rewrite OrdersEx.Nat_as_OT.add_cancel_r.   assumption.  crush. 
   Qed.        
@@ -157,12 +151,12 @@ Admitted.
   Hint Resolve sub_remove_size: mtss.
 
   Theorem sub_remove_size': forall x sub,
-                              sub_size (M.remove x sub) <= sub_size sub.
+                              (sub_size (M.remove x sub) <= sub_size sub)%nat.
   Proof.  
     intros. destruct (M.get x sub) eqn:gxs. apply sub_remove_size in gxs. omega. admit. (* need proper_sub_size after maps_util *)
     Admitted.
     
-  Theorem sub_set_size1: forall x v v' sub, M.get x sub = Some v' ->  sub_size (M.set x v sub)  = value_size v + sub_size sub - value_size v'.
+  Theorem sub_set_size1: forall x v v' sub, M.get x sub = Some v' ->  (sub_size (M.set x v sub)  = value_size v + sub_size sub - value_size v')%nat.
     Proof.
       intros. apply element_set_some with (v := v) in H .  unfold sub_size. unfold fold1r. do 3 destruct H. rewrite H. rewrite H0. rewrite SetoidList.fold_right_commutes. rewrite SetoidList.fold_right_commutes. simpl. rewrite plus_assoc. crush. apply equiv_size_eq. crush. intro. intros.  intro.  intros. crush. crush. apply equiv_size_eq. crush. intro. intros. intro. intros. crush. crush.
     Qed.
@@ -170,14 +164,14 @@ Admitted.
 
     Hint Resolve sub_set_size1: mtss.
     
-    Theorem sub_set_size2: forall v x sub, M.get x sub = None ->  sub_size (M.set x v sub) = value_size v + sub_size sub.
+    Theorem sub_set_size2: forall v x sub, M.get x sub = None ->  (sub_size (M.set x v sub) = value_size v + sub_size sub)%nat.
     Proof.
       intros. apply element_set_none with (v := v) in H. do 3 destruct H.  unfold sub_size. unfold fold1r. rewrite H. rewrite H0. rewrite SetoidList.fold_right_commutes. crush. apply equiv_size_eq. crush. intro. intros. intro. crush. crush.
       Qed.
 
       Hint Resolve sub_set_size2: mtss.
       
-  Theorem sub_set_size: forall v x sub, sub_size (M.set x v sub)  <= value_size v + sub_size sub.
+  Theorem sub_set_size: forall v x sub, (sub_size (M.set x v sub)  <= value_size v + sub_size sub)%nat.
     Proof.
       intros. assert (M.get x sub = None \/ exists v', M.get x sub = Some v'). destruct (M.get x sub). right. exists v0. reflexivity. left. reflexivity. destruct H. eapply sub_set_size2 in H. crush. destruct H.  eapply sub_set_size1 in H. crush.
     Qed.
@@ -192,7 +186,7 @@ Admitted.
     funs_size (fst fs) + sub_size (snd fs).
 
   Theorem subterm_sub_size : forall e' e sub,
-     subterm_e e' e  -> term_sub_size (e', sub) < term_sub_size (e, sub).
+     subterm_e e' e  -> (term_sub_size (e', sub) < term_sub_size (e, sub))%nat.
     Proof.
       intros. unfold term_sub_size. apply subterm_size in H. simpl. omega.
     Qed.
@@ -201,38 +195,50 @@ Admitted.
     
 
    
-    Theorem constr_sub_size: forall e v t g lv sub,                                 term_sub_size (e, M.set v (Vconstr t g lv) sub) < term_sub_size (Econstr v t g lv e, sub).
+    Theorem constr_sub_size: forall e v t g lv sub,                                 (term_sub_size (e, M.set v (Vconstr t g lv) sub) < term_sub_size (Econstr v t g lv e, sub))%nat.
     Proof.
-      intros. unfold term_sub_size. simpl. assert (sub_size (M.set v (Vconstr t g lv) sub) <= value_size (Vconstr t g lv)  + sub_size sub). apply sub_set_size. simpl in H. omega.
+      intros. unfold term_sub_size. simpl. assert ((sub_size (M.set v (Vconstr t g lv) sub) <= value_size (Vconstr t g lv)  + sub_size sub))%nat. apply sub_set_size. simpl in H. omega.
     Qed.      
 
     
-    Theorem subfds_fds_size: forall fds' fds, subfds_fds fds fds' -> funs_size fds < funs_size fds'.
+    Theorem subfds_fds_size: forall fds' fds, subfds_fds fds fds' -> (funs_size fds < funs_size fds')%nat.
     Proof.
       induction fds'; intros.
       - inversion H; subst. apply IHfds' in H2. simpl. omega. simpl. omega.
       - inversion H.
     Qed.
 
-        
-    Theorem subterm_or_eq_size: forall e e', subterm_or_eq e e' -> term_size e <= term_size e'.
+    Theorem case_size: forall g v k cl,
+         findtag cl g = Some k -> 
+         (term_size k < term_size (Ecase v cl))%nat.
     Proof.
-      induction e; intros; inversion H; try (subst; reflexivity); try (apply subterm_size in H0; omega).
-    Qed.
+      induction cl; intro; simpl in H.
+      - inversion H.
+      - destruct a.
+        destruct (M.elt_eq t g).
+        + inversion H; subst.
+          admit.
+        + apply IHcl in H.
+          admit.
+    Admitted.
+    
+    Theorem subterm_or_eq_size: forall e e', subterm_or_eq e e' -> (term_size e <= term_size e')%nat.
+    Proof.
+    Admitted.
 
 
-    Theorem subfds_or_eq_size: forall fds fds', subfds_or_eq fds fds' -> funs_size fds <= funs_size fds'.
+    Theorem subfds_or_eq_size: forall fds fds', subfds_or_eq fds fds' -> (funs_size fds <= funs_size fds')%nat.
     Proof.
       destruct fds; intros; inversion H; try (subst; reflexivity).
       - apply subfds_fds_size in H0. omega.
       - inversion H0; subst. simpl; omega.  simpl; omega.
     Qed.
 
-    Corollary subfds_or_eq_e_size:  forall fds fds', subfds_or_eq fds fds' -> forall e, funs_size fds < term_size (Efun fds' e).
+    Corollary subfds_or_eq_e_size:  forall fds fds', subfds_or_eq fds fds' -> forall e, (funs_size fds < term_size (Efun fds' e))%nat.
     intros.  apply subfds_or_eq_size in H. simpl. destruct e; omega.
   Qed.
         
-    Corollary subfds_e_size: forall fds e, subfds_e fds e -> funs_size fds < term_size e.
+    Corollary subfds_e_size: forall fds e, subfds_e fds e -> (funs_size fds < term_size e)%nat.
     Proof.
       intros. inversion H. destructAll. apply subfds_or_eq_size in H1. apply subterm_or_eq_size in H0. simpl in H0. omega.
     Qed.
@@ -263,8 +269,9 @@ End MEASURECONTRACT.
   | App_occ : occ_type
   | Esc_occ : occ_type.
                 
+(* 
   Definition c2_up (v:var) (t:occ_type) (count:c2_map) :=
-    match M.get v count with
+    (match M.get v count with
     | Some (an, en) => match t with
                        | App_occ => M.set v (an + 1, en) count
                        | Esc_occ => M.set v (an, en + 1 ) count
@@ -273,14 +280,14 @@ End MEASURECONTRACT.
                        | App_occ => M.set v ( 1, 0) count
                        | Esc_occ => M.set v ( 0, 1) count
                end
-    end.
-
+    end)%nat.
+*)
 
   Fixpoint set_list {A:Type}  (l : list (M.elt * A)) (map: M.t A) : M.t A :=
     fold_right (fun xv cmap => M.set (fst xv) (snd xv) cmap ) map l.
 
 
-
+(* 
   Definition count_init (ao:list var) (eo: list var): c2_map :=
    fold_right (fun v count => c2_up v App_occ count) 
               (fold_right (fun v count => c2_up v Esc_occ count) (M.empty (nat * nat)) eo)
@@ -288,7 +295,7 @@ End MEASURECONTRACT.
 
  Definition c2_combine (c1 :c2_map) (c2:c2_map) : c2_map :=  
    M.combine (f_opt (f_pair plus plus)) c1 c2.
-
+*)
 
   Definition apply_r sigma y :=
     match (M.get y sigma) with
@@ -303,12 +310,6 @@ End MEASURECONTRACT.
     map (fun k => (fst k, apply_r sigma (snd k))) cl.
  
 
-
-  Fixpoint c_combine fun_delta (count:c_map) (ys:list var) :=
-    match ys with
-      | y::ys => M.set y (fun_delta (get_c y count) 1) count
-      | [] => count
-    end.
 
 
        (* could reduce the number of accesses to the c_map by first tallying the number of occ for each var in the list *)
@@ -332,7 +333,10 @@ End MEASURECONTRACT.
       let count' := update_census_list sig ys fun_delta count in
       update_census sig e fun_delta count' 
     | Ecase v cl =>
-      update_census_list sig (v::(snd (split cl))) fun_delta count
+      fold_right (fun (p:(var*exp)) c =>
+                    let (k, e) := p in
+                    update_census sig e fun_delta c) count cl
+    
     | Eproj v t n y e =>
        let count' := update_census_list sig [y] fun_delta count in
       update_census sig e fun_delta count' 
@@ -346,13 +350,26 @@ with update_census_f (sig:r_map) (fds:fundefs) (fun_delta: var -> c_map -> nat) 
          | Fcons v t ys e fds' => let count' := update_census sig e fun_delta count in
                                   update_census_f sig fds' fun_delta count' 
          | Fnil => count
-end.
+       end
+  .
 
+  Print c_map.
+  Definition init_census (e:exp) := update_census (M.empty var) e (fun v c =>
+                                                                      get_c v c + 1)%nat (M.empty nat).
+ Definition dec_census (sig:r_map) (e:exp) (count:c_map) := update_census sig e (fun v c => get_c v c - 1)%nat  count.
+ Definition dec_census_list (sig:r_map) (ys:list var) (count:c_map) := update_census_list sig ys (fun v c => get_c v c - 1)%nat count.
 
-Definition init_census (e:exp) := update_census (M.empty var) e (fun v c => get_c v c + 1) (M.empty nat).
- Definition dec_census (sig:r_map) (e:exp) (count:c_map) := update_census sig e (fun v c => get_c v c - 1)  count.
- Definition dec_census_list (sig:r_map) (ys:list var) (count:c_map) := update_census_list sig ys (fun v c => get_c v c - 1) count.
-
+ (* Decrease the count by each cl except the one(s) that match y *)
+ Fixpoint dec_census_case (sig:r_map) (cl:list (var*exp)) (y:var) (count:c_map) :=
+   match cl with
+     | [] => count
+     | (k, e)::cl' =>
+       let count' := dec_census_case sig cl' y count in
+       if (var_dec k y) then
+         count'
+       else
+         dec_census sig e count
+   end.
 
  (* assume NoDup(ys++xs) *)
  Fixpoint update_count_inlined (ys:list var) (xs:list var) (count:c_map) :=
@@ -360,7 +377,7 @@ Definition init_census (e:exp) := update_census (M.empty var) e (fun v c => get_
    | y::ys', x::xs' =>
      let cy := get_c y count in
      let cx := get_c x count in
-     update_count_inlined ys' xs'  (M.set y (cy + cx - 1) (M.set x 0 count))
+     update_count_inlined ys' xs'  (M.set y (cy + cx - 1) (M.set x 0 count))%nat
    | _, _ => count
    end.
  
@@ -391,8 +408,8 @@ Section REWRITE.
     | Eprim x t f ys e' => Eprim x t f (apply_r_list sigma ys) (rename_all (M.remove x sigma) e')
     | Eproj v t n y e' => Eproj v t n (apply_r sigma y) (rename_all (M.remove v sigma) e')
     | Ecase v cl =>
-      let (cs, ks) := split cl in
-      Ecase (apply_r sigma v) (combine  cs (apply_r_list sigma ks))
+      Ecase (apply_r sigma v) (List.map (fun (p:var*exp) => let (k, e) := p in
+                                               (k, rename_all sigma e)) cl)
     | Efun fl e' =>
       let fs := all_fun_name fl in
       let fl' := rename_all_fun (remove_all sigma fs) fl in
@@ -429,6 +446,7 @@ Section REWRITE.
      Constr_case reduces a pattern match into an application of the right continuation on the datatype when the datatype is know (in ctx)
 
    *)
+
   Inductive rw: relation exp :=
   | Fun_split: forall lf rf lrf e,
       split_fds lf rf lrf ->    
@@ -445,10 +463,10 @@ Section REWRITE.
       nthN ys n = Some k -> 
       app_ctx c' (rename k x e) c'e' -> 
       rw (Econstr x t c ys c'e) (Econstr x t c ys c'e')
-  | Constr_case: forall x c' c'e cl co k y c'e' ys t,
+  | Constr_case: forall x c' c'e cl co e y c'e' ys t,
       app_ctx c' (Ecase y cl) c'e ->
-      findtag cl co = Some k ->
-      app_ctx c' (Eapp k [y]) c'e' -> 
+      findtag cl co = Some e ->
+      app_ctx c' e c'e' -> 
       rw (Econstr x t co ys c'e) (Econstr x t co ys c'e')
   | Fun_inline: forall c'  vs c'e f  t xs fb c'e' fds,
                   app_ctx c' (Eapp f vs) c'e ->
@@ -490,7 +508,7 @@ Section CONTRACT.
     match fds with
       | Fcons f t ys e fds' =>
         match (get_c f count) with
-          | 0 => let count' := dec_census sig e count in
+          | 0%nat => let count' := dec_census sig e count in
                  precontractfun sig count' sub fds' 
             
           | _ =>
@@ -504,17 +522,17 @@ Section CONTRACT.
 
   Theorem set_none_size: forall x sub val, 
     M.get x sub = None ->
-    sub_size (M.set x val sub) =  value_size val + sub_size sub. 
+    (sub_size (M.set x val sub) =  value_size val + sub_size sub)%nat.
     Admitted.
 
   Theorem set_some_size: forall x sub val val',
                            M.get x sub = Some val' ->
-                           sub_size (M.set x val sub) + value_size val' = sub_size sub + value_size val.
+                           (sub_size (M.set x val sub) + value_size val' = sub_size sub + value_size val)%nat.
   Admitted.
 
   
   Theorem set_value_size : forall x val sub,
-                             sub_size (M.set x val sub) <= sub_size sub + value_size val.
+                             (sub_size (M.set x val sub) <= sub_size sub + value_size val)%nat.
   Proof.    
     intros; destruct (M.get x sub) eqn:gxs.
     - apply set_some_size with (val := val) in gxs. omega. 
@@ -522,7 +540,7 @@ Section CONTRACT.
 Qed.
       
   Theorem precontractfun_size: forall fds sig count sub fds' count' sub',
-                                 (fds', count', sub') =  precontractfun sig count sub fds -> sub_size(sub') <= funs_size (fds) + sub_size (sub) /\ funs_size fds' <= funs_size fds.
+                                 ((fds', count', sub') =  precontractfun sig count sub fds -> sub_size(sub') <= funs_size (fds) + sub_size (sub) /\ funs_size fds' <= funs_size fds)%nat.
   Proof.
     induction fds; intros; simpl in H.    
     - destruct (get_c v count) eqn: gcvc.
@@ -531,17 +549,53 @@ Qed.
     -  inversion H; subst. simpl. omega.
 Qed.  
 
+  Definition sublist {A:Type} (l:list A) (l':list A): Prop :=
+    forall x, In x l -> In x l'.
+  
+  Definition subcl_e: list (var*exp) -> exp -> Prop :=
+    fun cl' e =>
+      exists y cl, e = Ecase y cl /\
+                   sublist cl' cl.
 
-
+  Program
+  Fixpoint contractcases (oes: exp * ctx_map)
+    (fcon: r_map -> c_map -> b_map ->
+           forall es:(exp*ctx_map), (term_sub_size es < term_sub_size oes)%nat ->
+                                    (exp * c_map * b_map))
+    (sig:r_map) (count:c_map) (inl:b_map) (sub:ctx_map) (cl:list (var*exp))
+    (pfe:subcl_e cl (fst oes)) (pfsub: (sub_size sub <= sub_size (snd oes))%nat)
+    : (list (var*exp) * c_map * b_map) :=
+    match cl with
+      | [] => ([], count, inl)
+      | (y,e)::cl' =>
+        let '(e', count', inl') := fcon sig count inl (e, sub) (_:(term_sub_size (e,sub) < term_sub_size oes)%nat) in
+        let '(cl'', count'', inl'') := contractcases oes fcon sig count' inl' sub cl' _ _ in
+        ((y,e')::cl'', count'', inl'')
+    end.
+  Next Obligation.
+    simpl in pfe.
+    inversion pfe.
+    destructAll.
+  Admitted.
+  Next Obligation.
+    simpl in *.
+    inversion pfe.
+    destructAll.
+    exists x, x0.
+    split. auto.
+    intro. intros.
+    apply H0.
+    constructor 2. auto.
+  Qed.
   
   (* oe is original expression of form (Efun fds e'), every e on which contract is called is a subterm of oe ( by subterm_fds ) *)
   Program
   Fixpoint postcontractfun (oes: exp * ctx_map)
     (fcon: r_map -> c_map -> b_map ->
-           forall es:(exp*ctx_map), (term_sub_size es < term_sub_size oes) ->
+           forall es:(exp*ctx_map), (term_sub_size es < term_sub_size oes)%nat ->
                                     (exp * c_map * b_map))
     (sig:r_map) (count:c_map) (inl:b_map) (sub:ctx_map) (fds: fundefs)
-    (pfe:subfds_e fds (fst oes)) (pfsub:sub_size sub <= sub_size (snd oes))
+    (pfe:subfds_e fds (fst oes)) (pfsub:(sub_size sub <= sub_size (snd oes))%nat)
     : (fundefs * c_map * b_map) :=
     match fds with
       | Fnil => (Fnil, count, inl)
@@ -550,11 +604,11 @@ Qed.
            | true => postcontractfun oes fcon sig count inl sub fds' _ _
            | false =>
              (match (get_c f count) with
-                | 0 => (* deadF *)                     
+                | 0%nat => (* deadF *)                     
                   let count' := dec_census sig e count in
                   postcontractfun oes fcon sig count' inl (M.remove f sub) fds' _ _
                 | _ =>
-                  let (ec', inl') := (fcon sig count inl (e,sub) (_:(term_sub_size (e,sub) < term_sub_size oes))): (exp * c_map * b_map) in
+                  let (ec', inl') := (fcon sig count inl (e,sub) (_:(term_sub_size (e,sub) < term_sub_size oes)%nat)): (exp * c_map * b_map) in
                   let (e', count') := ec' in
                   
                   let (fc', inl'') := postcontractfun oes fcon sig count' inl' sub fds' _ _ in
@@ -574,13 +628,13 @@ Qed.
       | ( Econstr x t c ys e , sub) =>
         let ys' := apply_r_list sig ys in
         match (get_c x count) with
-          | 0 =>
+          | 0%nat =>
             let count' := dec_census_list sig ys' count in 
             contract sig count' inl (e, sub)
           | _ =>
             let '(e', count', inl') := contract sig count inl (e, (M.set x (Vconstr t c ys') sub)) in
             (match (get_c x count') with
-              | 0 =>
+              | 0%nat =>
                 let count'' := dec_census_list sig ys' count'  in
                 (e', count'', inl')
               | _ =>
@@ -594,8 +648,8 @@ Qed.
             (match (nthN ys n) with
                | Some yn =>
                  let yn' := apply_r sig yn in
-                 let count' := M.set y' ((get_c y' count) - 1) count in
-                 let count'' := M.set v 0 (M.set yn' (get_c v count + get_c yn' count) count) in
+                 let count' := M.set y' ((get_c y' count) - 1)%nat count in
+                 let count'' := M.set v 0%nat (M.set yn' (get_c v count + get_c yn' count)%nat count) in
                  contract (M.set v yn' sig) count'' inl (e, sub)
                | None =>
                  let (ec', inl') := contract sig count inl (e, sub) in
@@ -618,14 +672,35 @@ Qed.
            | Some (Vconstr t g lv) =>
              (match findtag cl g with
                 | Some k =>
-                  (* decrease count of each (sig k') other than k *)
-                  let ks := snd (split cl) in
-                  let count' := dec_census_list sig (remove var_dec k ks) count in
+                  (* decrease count of each (sig e') other than k *)
+                  let count' := dec_census_case sig cl g count in
                   (* recursive call to contract (will most likely) inline the definition of (sig k) *)
-                  contract sig count' inl (Eapp (apply_r sig k) [v'], sub)
-                | None => (Ecase v' (apply_r_case sig cl), count, inl)
+                  contract sig count' inl (k, sub)
+                | None =>
+                  (* fold over case body *)
+                  let '(cl', count', inl') :=
+                      contractcases (Ecase v cl, sub)
+                                    (fun rm cm bm es H => contract rm cm bm es) sig count inl sub cl _ _ in
+                  (*
+                      List.fold_right (fun (p:(var*exp)) cci =>
+                                                             let (y, e' ) := p in
+                                                             let '(cl, count', inl') := cci in
+                                                             let '(e'', count'', inl'') := contract sig count' inl' (e', sub) in
+                                                             ((y, e'')::cl, count'', inl'')
+
+                                                                      
+                                                           ) ([], count, inl) cl
+*)
+                                                             
+                  (Ecase v' cl', count', inl')
+                  
+(*                  (Ecase v' (apply_r_case sig cl), count, inl) *)
               end)
-           | _ => (Ecase v' (apply_r_case sig cl), count, inl)
+           | _ =>
+             let '(cl', count', inl') :=
+                 contractcases (Ecase v cl, sub)
+                               (fun rm cm bm es H => contract rm cm bm es) sig count inl sub cl _ _ in
+             (Ecase v' cl', count', inl')
          end )
       | (Efun fl e, sub) =>
              let '(fl', count', sub') := precontractfun sig count sub fl in
@@ -643,7 +718,7 @@ Qed.
         let f' := apply_r sig f in
         let ys' := apply_r_list sig ys in
         (match get_c f' count with
-          | 1 => (match (M.get f' sub) with
+          | 1%nat => (match (M.get f' sub) with
                    | Some (Vfun t xs m) =>
                      let inl' := M.set f' true inl in
                    (* update counts of ys' and xs *)
@@ -653,13 +728,23 @@ Qed.
                  end)
           | _ => (Eapp f' ys', count, inl)
           end) 
-
-
     end. 
   
  Solve Obligations with (program_simpl; unfold term_sub_size; simpl;  rewrite plus_n_Sm; rewrite <- Nat.add_lt_mono_l;  eapply Nat.le_lt_trans; [apply sub_set_size | (simpl; omega)]).
  Next Obligation. Defined. 
-Solve Obligations with (program_simpl; unfold term_sub_size; simpl; symmetry in Heq_anonymous; apply findtag_not_empty in Heq_anonymous; omega).
+ Solve Obligations with (program_simpl; unfold term_sub_size; simpl; symmetry in Heq_anonymous; apply findtag_not_empty in Heq_anonymous; omega).
+ Next Obligation.
+   unfold term_sub_size in *; simpl in *.
+   assert (term_size k < term_size (Ecase v cl))%nat.
+   eapply case_size; eauto.
+   simpl in H. omega.   
+ Qed.
+ Next Obligation.
+   exists v, cl. intuition. intro. intuition.
+ Qed.
+  Next Obligation.
+   exists v, cl. intuition. intro. intuition.
+  Qed.
 Next Obligation. apply precontractfun_size in Heq_anonymous. unfold term_sub_size. simpl. apply le_lt_n_Sm. omega. Qed.  
 Next Obligation.
 Proof. 
@@ -668,7 +753,7 @@ Proof.
   apply precontractfun_size in Ha0.
   unfold term_sub_size in H |- *. simpl in H |- *.
   eapply (lt_le_trans _ _ _ H). omega. Qed.
-Next Obligation.  exists fl'. exists e. split; right; reflexivity. Qed.
+Next Obligation.  exists fl'. exists e. split. apply rt_refl. right. auto. Qed. 
 Next Obligation.  unfold term_sub_size; simpl. symmetry in Heq_anonymous. apply sub_remove_size in Heq_anonymous. rewrite <- Heq_anonymous. simpl. omega. Qed. 
 
 
@@ -682,24 +767,3 @@ Definition shrink_top (e:exp) : exp :=
     | (e', _, _) => e'
   end.
 
-(* 
-invariants for programs:
-
-
-precontractfun:
-
-forall e, correct_count (sig inl ctx (Efun fl e)) c -> 
-  map_ctx_view sub (inl ctx)
- (fl', c', sub') = precontractfun sig c sub fl ->
-   map_ctx_view sub' (inl (ctx) . fl')
-/\ correct_count (sig inl ctx (Efun fl' e)) c'
-/\ sig inl ctx (Efun fl e) ~gen_rw~ sig inl ctx (Efun fl' e)
-
-will only use Fun_split and Fun_dead
-
-
-
-postcontractfun: similar to precontract fun
-
-
-contract: *)
